typeclass instance for Fintype (Set a) + required theorems about List.power_upto, restructured files

FormaleSystemeInLean/LectureAndExercise/ideas.lean
@@ -2,13 +2,6 @@ import FormaleSystemeInLean.LectureAndExercise.lecture1
 
 set_option linter.unusedSectionVars false
 
--- inspired by mathlib
-class Fintype (α : Type u) where
-  elems : List α
-  complete : ∀ a : α, a ∈ elems
-
-def List.toSet (l : List α) : Set α := fun e => e ∈ l
-
 def l0 : List (List Nat) := []
 def l1 : List (Nat) := [0, 1, 2]
 def l2 : List (List Nat) := [[]]
@@ -38,12 +31,6 @@ def List.power (l : List α) : List (List α) :=
     | n+1 => let prev := loop n; prev ++ (prev.flatMap (fun l' => l.map fun e => e:: l'))
   loop l.length
 
-def List.power_upto (l : List α) (n : Nat) : List (List α) :=
-  let rec loop : Nat → List (List α)
-    | 0 => [[]]
-    | n+1 => let prev := loop n; prev ++ (prev.flatMap (fun l' => l.map fun e => e:: l'))
-  loop n
-
 def List.powerset_lists [BEq α] (l : List α) : List (List α) :=
   (List.powerRec l l.length).eraseDups
 
@@ -58,121 +45,35 @@ def List.powerset_lists [BEq α] (l : List α) : List (List α) :=
 #eval [2, 3].power
 #eval [1, 2, 3, 4, 5, 6, 7].power.eraseDups
 #eval [1, 2, 3].power'.eraseDups.length -/
-#eval [0, 1, 2].power_upto 3
+#eval ([0, 1, 2].power_upto 3).eraseDups
 #eval l0.power_upto 99
 
-theorem nil_power (n : Nat) (l : List α) : l = [] -> l.power_upto n = [[]] := by
-  intro l_eq
-  induction n with
-  | zero =>
-    unfold List.power_upto List.power_upto.loop
-    rfl
-  | succ n ih =>
-    unfold List.power_upto List.power_upto.loop
-    subst l
-    simp -- mit was?
-    unfold List.power_upto at ih
-    rw [ih]
-    simp
-
-theorem elem_power (T : Fintype α) (l : List α) (n : Nat) : n ≤ T.elems.length → l.length = n → l ∈ T.elems.power_upto n := by
-  intro n_le l_len
-  cases h : T.elems with
-  | nil =>
-    rw [nil_power]
-    . cases l with
-    | nil =>
-      grind
-    | cons a s =>
-      cases n with
-      | zero =>
-        grind
-      | succ n =>
-        rw [List.mem_singleton]
-        exfalso
-        have elems_length : T.elems.length = 0 := by
-          rw [List.eq_nil_iff_length_eq_zero] at h
-          exact h
-        rw [elems_length] at n_le
-        contradiction
-    . rfl
-  | cons b s =>
-    induction n generalizing l with
-    | zero =>
-      unfold List.power_upto List.power_upto.loop
-      have l_eq : l = [] := by
-        rw [List.eq_nil_iff_length_eq_zero]
-        exact l_len
-      rw [l_eq]
-      grind
-    | succ n ih =>
-      unfold List.power_upto List.power_upto.loop
-      simp
-      have l_neq_nil : l ≠ [] := by
-        have l_len_gz : l.length > 0 := by
-          rw [← Nat.succ_eq_add_one] at l_len
-          grind
-        rw [List.ne_nil_iff_length_pos]
-        exact l_len_gz
-      have l_eq : ∃ a l', l = a::l' ∧ l'.length = n := by
-        rw [List.ne_nil_iff_exists_cons] at l_neq_nil
-        rcases l_neq_nil with ⟨a, l', l_eq⟩
-        exists a, l'
-        constructor
-        . exact l_eq
-        . grind
-      rcases l_eq with ⟨a, l', l_eq, l'_len⟩
-      have aux : n ≤ T.elems.length := by grind
-      apply Or.inr
-      exists l'
-      constructor
-      . apply ih l' aux l'_len
-      . by_cases ha : a = b
-        . apply Or.inl
-          rw [← ha]
-          exact l_eq
-        . apply Or.inr
-          exists a
-          constructor
-          . have a_mem : a ∈ b::s := by
-              have complete := T.complete
-              specialize complete a
-              rw [h] at complete
-              exact complete
-            grind
-          symm
-          exact l_eq
-
-theorem set_of_list (T : Fintype α) (S : Set α) [DecidablePred S] : ∃ (l : List α), l.toSet = S := by
+theorem max_card (T : Fintype α) (S : Set α) [BEq α] [DecidablePred S] : S.toList.length ≤ T.elems.length := by
   have complete := T.complete
-  exists T.elems.filter (fun a => a ∈ S)
-  apply Set.ext
-  intro a
-  constructor
-  . intro a_mem
-    unfold List.toSet at a_mem
-    simp only [Membership.mem] at a_mem
+  cases ht:  T.elems with
+  | nil =>
+    rw [ht] at complete
+    simp only [List.mem_nil_iff] at complete
+    rw [List.length_nil, Nat.le_zero]
 
     sorry
-  . intro a_mem
-    unfold List.toSet
-    simp only [Membership.mem]
+  | cons b a =>
+    -- entweder S.toList.length = (b::a).length
+    -- oder...
+    rw [Nat.le_iff_lt_or_eq]
+    by_cases hs : S.toList.length = (b :: a).length
+    . apply Or.inr
+      exact hs
+    . simp only [hs]
+      apply Or.inl
 
+      sorry
 
-    sorry
-
-instance (T : Fintype α) [BEq α] : Fintype (Set α) where
-  elems := (T.elems.power_upto T.elems.length).map (fun x => x.toSet)
-  complete := by
-    intro S
-
-    sorry
-
-def Set.map (f : α → β) (S : Set α) [Fintype α] : Set β :=
-  fun b => ∃ (a : α), a ∈ S ∧ f a = b
-
-def Set.toList (S : Set α) [DecidablePred S] [Fintype α] : List α :=
-  Fintype.elems.filter (· ∈ S)
+-- daraus soll DecidablePred S folgen
+theorem set_of_list (T : Fintype α) (S : Set α) : ∃ (l : List α), l.toSet = S := by
+  have complete := T.complete
+  --exists (fun a => a ∈ l).toSet
+  sorry
 
 structure DFA (Q : Type u) (Sigma : Type v) [Fintype Q] where
   𝓠 : Set Q
