FormaleSystemeInLean/LectureAndExercise/set_powertype.lean
@@ -1,0 +1,242 @@
+
+-- inspired by mathlib
+class Fintype (α : Type u) where
+  elems : List α
+  complete : ∀ a : α, a ∈ elems
+
+def Set (α : Type u) := α -> Prop
+
+def Set.elem (S : Set α) (a : α) [DecidablePred S] : Bool :=
+  decide (S a)
+
+def Set.toList (S : Set α) [Fintype α] [DecidablePred S] : List α :=
+  Fintype.elems.filter (fun x => S.elem x)
+
+-- The following type class instances are just allowing us to use some basic notation like ∅, ∈ or ∪ with the right definitions..
+instance : EmptyCollection (Set α) where
+  emptyCollection := fun _ => False
+
+instance : Membership α (Set α) where
+  mem S a := S a
+
+instance : Union (Set α) where
+  union A B := fun e => e ∈ A ∨ e ∈ B
+
+instance : Inter (Set α) where
+  inter A B := fun e => e ∈ A ∧ e ∈ B
+
+instance : HasSubset (Set α) where
+  Subset A B := ∀ e, e ∈ A -> e ∈ B
+
+instance : HasSSubset (Set α) where
+  SSubset A B := A ⊆ B ∧ ¬ B ⊆ A
+
+instance : SDiff (Set α) where
+  sdiff A B := fun e => e ∈ A ∧ ¬(e ∈ B)
+
+def Set.powerset (α : Type u) (S : Set α) := fun x => x ⊆ S
+
+def Set.map (f : α → β) (S : Set α) [Fintype α] : Set β :=
+  fun b => ∃ (a : α), a ∈ S ∧ f a = b
+
+-- Set extensionality: Two sets are equal if they contain the same elements. This is not something we define but we can prove it!
+theorem Set.ext (X Y : Set α) : (∀ e, e ∈ X ↔ e ∈ Y) -> X = Y := by
+  intro h; apply funext; intro e; apply propext; specialize h e; exact h
+
+def Powertype (α : Type u) := Set α
+
+instance : Membership α (Powertype α) where
+  mem S a := S a
+
+def List.toSet (l : List α) : Set α := fun e => e ∈ l
+
+def List.power_upto (l : List α) (n : Nat) : List (List α) :=
+  let rec loop : Nat → List (List α)
+    | 0 => [[]]
+    | n+1 => let prev := loop n; prev ++ (prev.flatMap (fun l' => l.map fun e => e:: l'))
+  loop n
+
+theorem nil_power (n : Nat) (l : List α) : l = [] -> l.power_upto n = [[]] := by
+  intro l_eq
+  induction n with
+  | zero =>
+    unfold List.power_upto List.power_upto.loop
+    rfl
+  | succ n ih =>
+    unfold List.power_upto List.power_upto.loop
+    subst l
+    simp -- mit was?
+    unfold List.power_upto at ih
+    rw [ih]
+    simp
+
+theorem elem_power (T : Fintype α) (l : List α) (n : Nat) : n ≤ T.elems.length → l.length = n → l ∈ T.elems.power_upto n := by
+  intro n_le l_len
+  cases h : T.elems with
+  | nil =>
+    rw [nil_power]
+    . cases l with
+    | nil =>
+      grind
+    | cons a s =>
+      cases n with
+      | zero =>
+        grind
+      | succ n =>
+        rw [List.mem_singleton]
+        exfalso
+        have elems_length : T.elems.length = 0 := by
+          rw [List.eq_nil_iff_length_eq_zero] at h
+          exact h
+        rw [elems_length] at n_le
+        contradiction
+    . rfl
+  | cons b s =>
+    induction n generalizing l with
+    | zero =>
+      unfold List.power_upto List.power_upto.loop
+      have l_eq : l = [] := by
+        rw [List.eq_nil_iff_length_eq_zero]
+        exact l_len
+      rw [l_eq]
+      grind
+    | succ n ih =>
+      unfold List.power_upto List.power_upto.loop
+      simp
+      have l_neq_nil : l ≠ [] := by
+        have l_len_gz : l.length > 0 := by
+          rw [← Nat.succ_eq_add_one] at l_len
+          grind
+        rw [List.ne_nil_iff_length_pos]
+        exact l_len_gz
+      have l_eq : ∃ a l', l = a::l' ∧ l'.length = n := by
+        rw [List.ne_nil_iff_exists_cons] at l_neq_nil
+        rcases l_neq_nil with ⟨a, l', l_eq⟩
+        exists a, l'
+        constructor
+        . exact l_eq
+        . grind
+      rcases l_eq with ⟨a, l', l_eq, l'_len⟩
+      have aux : n ≤ T.elems.length := by grind
+      apply Or.inr
+      exists l'
+      constructor
+      . apply ih l' aux l'_len
+      . by_cases ha : a = b
+        . apply Or.inl
+          rw [← ha]
+          exact l_eq
+        . apply Or.inr
+          exists a
+          constructor
+          . have a_mem : a ∈ b::s := by
+              have complete := T.complete
+              specialize complete a
+              rw [h] at complete
+              exact complete
+            grind
+          symm
+          exact l_eq
+
+theorem inclusion_succ (T : Fintype α) (l : List α) (n : Nat) : l.length ≤ T.elems.length -> l ∈ T.elems.power_upto n -> l ∈ T.elems.power_upto (n+1) := by
+  intro l_len l_mem
+  unfold List.power_upto List.power_upto.loop
+  simp
+  apply Or.inl
+  exact l_mem
+
+theorem inclusion (T : Fintype α) (l : List α) (n : Nat) (m : Nat) : n ≤ m -> l ∈ T.elems.power_upto n -> l ∈ T.elems.power_upto m := by
+  intro le l_mem
+  induction le with
+  | refl =>
+    simp_all
+  | @step k b ih =>
+    unfold List.power_upto List.power_upto.loop
+    simp
+    apply Or.inl
+    exact ih
+
+theorem powerlist (T : Fintype α) (l : List α) : l.length ≤ T.elems.length -> l ∈ T.elems.power_upto T.elems.length := by
+  intro l_len
+  cases ht: T.elems with
+  | nil =>
+    rw [List.eq_nil_iff_length_eq_zero] at ht
+    simp only [List.length_nil]
+    unfold List.power_upto List.power_upto.loop
+    rw [ht, Nat.le_zero, ← List.eq_nil_iff_length_eq_zero] at l_len
+    rw [l_len, List.mem_singleton]
+  | cons b s =>
+    have aux := inclusion_succ T l l.length l_len
+    have aux2 := elem_power T l l.length l_len rfl
+    rw [ht, List.length_cons, Nat.le_add_one_iff] at l_len
+    rcases l_len with inl | inr
+    . have test := aux aux2
+      rw [ht] at test
+      rw [List.length_cons]
+      have aux3 := inclusion T l l.length s.length inl aux2
+      unfold List.power_upto List.power_upto.loop
+      simp
+      apply Or.inl
+      rw [← ht]
+      exact aux3
+    . rw [inr, ht] at aux2
+      rw [List.length_cons]
+      exact aux2
+
+theorem exists_mem_powertype (T : Fintype α) (S : Set α) [BEq α] [DecidablePred S] : ∃ (l : List α), l = S.toList ∧ l ∈ (T.elems.power_upto T.elems.length)  := by
+  exists S.toList
+  constructor
+  . rfl
+  . have l_len : S.toList.length ≤ T.elems.length := by
+      unfold Set.toList
+      apply List.length_filter_le
+    have mem := powerlist T S.toList l_len
+    exact mem
+
+instance (S : Set α) [Fintype α] : DecidablePred S := by
+
+  sorry
+
+theorem elem_iff_mem (S : Set α) (a : α) [Fintype α] : S.elem a = true ↔ a ∈ S := by
+  unfold Set.elem
+  simp only [Membership.mem]
+  grind
+
+theorem toList_toSet (l : List α) (S : Set α) (T : Fintype α) : l = S.toList → S = l.toSet := by
+  intro eq
+  apply Set.ext
+  intro e
+  constructor
+  . intro e_mem
+    unfold List.toSet
+    unfold Set.toList at eq
+    rw [eq]
+    simp --only [Membership.mem, Set.elem]
+    constructor
+    . have complete := T.complete
+      specialize complete e
+      exact complete
+    . rw [elem_iff_mem]
+      . exact e_mem
+  . intro e_mem
+    unfold List.toSet at e_mem
+    rw [eq] at e_mem
+    unfold Set.toList at e_mem
+    simp_all --only [Membership.mem, Set.elem] at e_mem
+    rcases e_mem with ⟨e_mem, e_elem⟩
+    rw [elem_iff_mem] at e_elem
+    exact e_elem
+
+instance (T : Fintype α) [BEq α] : Fintype (Set α) where
+  elems := (T.elems.power_upto T.elems.length).map (fun x => x.toSet)
+  complete := by
+    intro S
+    have exists_l := exists_mem_powertype T S
+    rcases exists_l with ⟨l, l_eq, l_mem⟩
+    rw [List.mem_map]
+    exists l
+    constructor
+    . exact l_mem
+    . have aux := toList_toSet l S T l_eq
+      symm at aux
+      exact aux
